Add refinement rules

examples/02-proof-rules/RefinementRules.v
@@ -9,55 +9,311 @@ Context {State1 State2 : Type}.
 (* TODO: Keep only the useful rules... *)
 
 (* ========================================================================== *)
-(* Refinement Mapping                                                         *)
+(* Utility definitions                                                        *)
+(* ========================================================================== *)
+
+(* Not from refs *)
+Definition util_inverse (r : State1 -> State2) (s2 : State2) (s1 : State1) : Prop :=
+    r s1 = s2.
+
+(* Not from refs *)
+Definition util_inverse0 (r : State1 -> State2 -> Prop) (s2 : State2) (s1 : State1) : Prop :=
+    r s1 s2.
+
+(* Not from refs *)
+Definition util_reflexive (f : State1 -> State1) : Prop :=
+    forall s1, f s1 = s1.
+
+(* Not from refs *)
+Definition util_reflexive0 (r: State1 -> State1 -> Prop) : Prop :=
+    forall s1, r s1 s1.
+
+(* Not from refs *)
+Definition util_symmetric (f : State1 -> State1) : Prop :=
+    forall s1, f (f s1) = s1.
+
+(* Not from refs *)
+Definition util_symmetric0 (r : State1 -> State1 -> Prop) : Prop :=
+    forall s1 s2, r s1 s2 -> r s2 s1.
+
+(* Not from refs *)
+Definition util_partial_function0 (r : State1 -> State2 -> Prop) : Prop :=
+    forall s1 s2 s3, r s1 s2 -> r s1 s3 -> s2 = s3.
+
+(* Not from refs *)
+(* The refinement mapping operator `RefinementMapping` but __not__ stuttering
+   closed *)
+Definition util_with2 {S1 S2 : Type} (f : S1 -> S2) (F : property S1) : property S2 :=
+    fun beh2 =>
+        exists beh1 : behavior S1,
+            (forall n : nat, f (beh1 n) = beh2 n)
+            /\ F beh1.
+
+(* Not from refs *)
+(* The refinement mapping operator `CoRefinementMapping` but __not__ stuttering
+   closed *)
+Definition util_co_with2 {S1 S2 : Type} (f : S1 -> S2) (F : property S1) : property S2 :=
+    fun beh2 =>
+        forall beh1 : behavior S1,
+            (forall n : nat, f (beh1 n) = beh2 n)
+            -> F beh1.
+
+(* Not from refs *)
+(* The refinement mapping operator `RefinementMapping0` but __not__ stuttering
+   closed *)
+Definition util_with02 {S1 S2 : Type} (r : S1 -> S2 -> Prop) (F : property S1) : property S2 :=
+    fun beh2 =>
+        exists beh1 : behavior S1,
+            (forall n : nat, r (beh1 n) (beh2 n))
+            /\ F beh1.
+
+(* Not from refs *)
+(* The refinement mapping operator `CoRefinementMapping0` but __not__ stuttering
+   closed *)
+Definition util_co_with02 {S1 S2 : Type} (r : S1 -> S2 -> Prop) (F : property S1) : property S2 :=
+    fun beh2 =>
+        forall beh1 : behavior S1,
+            (forall n : nat, r (beh1 n) (beh2 n))
+            -> F beh1.
+
+(* ========================================================================== *)
+(* Utility lemmas                                                             *)
+(* ========================================================================== *)
+
+(* Not from refs *)
+Lemma AUX1 (Op : property State1 -> property State2) (F G : property State1) :
+    (forall F G : property State1, valid (F \impl G) -> valid ((Op F) \impl (Op G))) ->
+        valid (Op (F \land G)
+            \impl (Op F) \land (Op G)).
+Proof.
+(* TODO *) Admitted. 
+
+(* Not from refs *)
+Lemma AUX2 (Op : property State1 -> property State2) (F_ : nat -> property State1) :
+    (forall F G : property State1, valid (F \impl G) -> valid ((Op F) \impl (Op G))) ->
+        valid (Op (\A i : F_ i)
+            \impl \A i : Op (F_ i)).
+Proof.
+(* TODO *) Admitted.
+
+(* ========================================================================== *)
+(* Refinement Mapping / 0                                                     *)
 (* ========================================================================== *)
 
 (* Note: not from references *)
-Lemma RM1 (f : State1 -> State2) (F G : property State1) :
-    valid (F \impl G)
-        -> valid ((F WITH f) \impl (G WITH f)).
+(* Refinement version of EE1 *)
+Lemma RM1 (f : State1 -> State1) (F : property State1) :
+    util_reflexive f ->
+        valid (F \impl (F WITH f)).
 Proof.
-    admit.
-Admitted.
+(* TODO *) Admitted.
 
 (* Note: not from references *)
-Corollary RM1COR1 (f: State1 -> State1) (F G : property State1) :
-    valid (G WITH f \impl G)
+(* Refinement version of EE1 *)
+Lemma R0M1 (r : State1 -> State1 -> Prop) (F : property State1) :
+    util_reflexive0 r ->
+        valid (F \impl (F WITH0 r)).
+Proof.
+(* TODO *) Admitted.
+
+(* Note: not from references *)
+(* Refinement version of EE2 *)
+Lemma RM2 (f: State1 -> State1) (F G : property State1) :
+    valid (G WITH f \impl G) (* cf. "x not free in G" with "x" as f in EE2 *)
         -> valid (F \impl G)
             -> valid (F WITH f \impl G).
 Proof.
-    admit.
-Admitted.
+(* TODO *) Admitted.
 
 (* Note: not from references *)
-Lemma RM2 (f : State1 -> State2) (F G : property State1) :
+(* Refinement version of EE2 *)
+Lemma R0M2 (r: State1 -> State1 -> Prop) (F G : property State1) :
+    valid (G WITH0 r \impl G) (* cf. "x not free in G" with "x" as f in EE2 *)
+        -> valid (F \impl G)
+            -> valid (F WITH0 r \impl G).
+Proof.
+(* TODO *) Admitted.
+
+(* Note: not from references *)
+(* Refinement version of EE3 *)
+Lemma RM3 (f : State1 -> State2) (F G : property State1) :
+    valid (F \impl G)
+        -> valid ((F WITH f) \impl (G WITH f)).
+Proof.
+(* TODO *) Admitted.
+
+(* Note: not from references *)
+(* Refinement version of EE3 *)
+Lemma R0M3 (r : State1 -> State2 -> Prop) (F G : property State1) :
+    valid (F \impl G)
+        -> valid ((F WITH0 r) \impl (G WITH0 r)).
+Proof.
+(* TODO *) Admitted.
+
+(* Note: not from references *)
+Lemma RM4 (f : State1 -> State2) (F G : property State1) :
     util_injective f ->
         util_stuttering_closed G ->
             valid ((F WITH f) \impl (G WITH f)) ->
                 valid (F \impl G).
 Proof.
-    admit.
-Admitted.
+(* TODO *) Admitted.
 
-(* ========================================================================== *)
-(* Refinement Mapping 0                                                       *)
-(* ========================================================================== *)
-
-(* Note: not from references *)
-Lemma R0M1 (r : State1 -> State2 -> Prop) (F G : property State1) :
-    valid (F \impl G)
-        -> valid ((F WITH0 r) \impl (G WITH0 r)).
+(* Not from refs *)
+Lemma RM5a (f : State1 -> State2) (F G : property State1) :
+    valid (((F \land G) WITH f)
+        \impl ((F WITH f) \land (G WITH f))).
 Proof.
-    admit.
-Admitted.
+(* TODO *) Admitted.
 
-(* Note: not from references *)
-Corollary R0M1COR1 (r: State1 -> State1 -> Prop) (F G : property State1) :
-    valid (G WITH0 r \impl G)
-        -> valid (F \impl G)
-            -> valid (F WITH0 r \impl G).
+(* Not from refs *)
+Lemma RM5b (f : State1 -> State2) (F_ : nat -> property State1) :
+    valid (((\A i : F_ i) WITH f)
+        \impl (\A i : (F_ i WITH f))).
 Proof.
-    admit.
-Admitted.
+(* TODO *) Admitted.
+
+Lemma RM5c (f : State1 -> State2) (F G : property State1) :
+    valid (((F WITH f) \land (G CO_WITH f))
+        \impl ((F \land G) WITH f)).
+Proof.
+(* TODO *) Admitted.
+
+(* Not from refs *)
+Lemma R0M5a (r : State1 -> State2 -> Prop) (F G : property State1) :
+    valid (((F \land G) WITH0 r)
+        \impl ((F WITH0 r) \land (G WITH0 r))).
+Proof.
+(* TODO *) Admitted.
+
+(* Not from refs *)
+Lemma R0M5b (r : State1 -> State2 -> Prop) (F_ : nat -> property State1) :
+    valid (((\A i : F_ i) WITH0 r)
+        \impl (\A i : (F_ i WITH0 r))).
+Proof.
+(* TODO *) Admitted.
+
+(* Not from refs *)
+Lemma R0M5c (r : State1 -> State2 -> Prop) (F G : property State1) :
+    valid (((F WITH0 r) \land (G CO_WITH0 r))
+        \impl ((F \land G) WITH0 r)).
+Proof.
+(* TODO *) Admitted.
+
+(* Frobenius reciprocity `->` direction *)
+(* Not from refs *)
+Lemma RM6a (r : State1 -> State2) (F : property State2) (G : property State1) :
+    util_stuttering_closed F ->
+        valid ((((F WITH0 (util_inverse r)) \land G) WITH r)
+            \impl (F \land (G WITH r))).
+Proof.
+(* TODO *) Admitted.
+
+(* Frobenius reciprocity `->` direction *)
+(* Not from refs *)
+Lemma R0M6a (f : State1 -> State2 -> Prop) (F : property State2) (G : property State1) :
+    util_partial_function0 f ->
+        util_stuttering_closed F ->
+            valid ((((F WITH0 (util_inverse0 f)) \land G) WITH0 f)
+                \impl (F \land (G WITH0 f))).
+Proof.
+(* TODO *) Admitted.
+
+(* Not from refs *)
+(* Frobenius reciprocity `<-` direction *)
+Lemma RM6b (r : State1 -> State2) (F : property State2) (G : property State1) :
+    valid ((F \land (G WITH r))
+        \impl (((F WITH0 (util_inverse r)) \land G) WITH r)).
+Proof.
+(* TODO *) Admitted.
+
+(* Not from refs *)
+(* Frobenius reciprocity `<-` direction *)
+Lemma R0M6b (f : State1 -> State2 -> Prop) (F : property State2) (G : property State1) :
+    valid ((F \land (G WITH0 f))
+        \impl (((F WITH0 (util_inverse0 f)) \land G) WITH0 f)).
+Proof.
+(* TODO *) Admitted.
+
+(* Not from refs *)
+Lemma RM7 (f : State1 -> State2) (F : property State1) (G : property State2) :
+    valid (F WITH f \impl G) <->
+        valid (F \impl (G CO_WITH0 (util_inverse f))).
+Proof.
+(* TODO *) Admitted.
+
+(* Not from refs *)
+Lemma R0M7 (f : State1 -> State2 -> Prop) (F : property State1) (G : property State2) :
+    valid (F WITH0 f \impl G) <->
+        valid (F \impl (G CO_WITH0 (util_inverse0 f))).
+Proof.
+(* TODO *) Admitted.
+
+(* Not from refs *)
+Lemma RM8 (f : State1 -> State2) (F : property State2) (G : property State1) :
+    valid (F WITH0 (util_inverse f) \impl G) <->
+        valid (F \impl (G CO_WITH f)).
+Proof.
+(* TODO *) Admitted.
+
+(* Not from refs *)
+Lemma R0M8 (f : State1 -> State2 -> Prop) (F : property State2) (G : property State1) :
+    valid (F WITH0 (util_inverse0 f) \impl G) <->
+        valid (F \impl (G CO_WITH0 f)).
+Proof.
+(* TODO *) Admitted.
+
+(* Not from refs *)
+Lemma RM9 (f : State1 -> State1) (G : property State1) :
+    util_symmetric f ->
+        valid ((G WITH f) \impl G) ->
+            valid (G \impl (G CO_WITH f)).
+Proof.
+(* TODO *) Admitted.
+
+(* Not from refs *)
+Lemma R0M9 (r : State1 -> State1 -> Prop) (G : property State1) :
+    util_symmetric0 r ->
+        valid ((G WITH0 r) \impl G) ->
+            valid (G \impl (G CO_WITH0 r)).
+Proof.
+(* TODO *) Admitted.
+
+(* Not from refs *)
+Lemma RM10a (f : State1 -> State2) (F : property State1) :
+    valid ((util_with2 f F) \impl (F WITH f)).
+Proof.
+(* TODO *) Admitted.
+
+(* Not from refs *)
+Lemma RM10b (f : State1 -> State2) (F : property State1) :
+    valid ((F CO_WITH f) \impl (util_co_with2 f F)).
+Proof.
+(* TODO *) Admitted.
+
+Lemma RM11a (f : State1 -> State2) (F : property State2) :
+    util_stuttering_closed F ->
+        valid ((F WITH0 (util_inverse f))
+            \impl (util_with02 (util_inverse f) F)).
+Proof.
+(* TODO *) Admitted.
+
+(* Not from refs *)
+Lemma RM11b (f : State1 -> State2) (F : property State2) :
+    util_stuttering_closed F ->
+        valid ((util_co_with02 (util_inverse f) F)
+            \impl (F CO_WITH0 (util_inverse f))).
+Proof.
+(* TODO *) Admitted.
+
+(* Not from refs *)
+Lemma RM12 (f : State1 -> State2) (Bl : property State1) (A B : property State2) :
+    util_stuttering_closed A ->
+        util_stuttering_closed B ->
+            valid (((util_with02 (util_inverse f) A) \land Bl)
+                \impl (util_co_with02 (util_inverse f) B)) ->
+                    valid ((A \land (Bl WITH f)) \impl B).
+Proof.
+(* TODO *) Admitted.
 
 End rules.
